src/vminus/CompilImpTest.v
@@ -1,0 +1,313 @@
+Require Import List.
+Import ListNotations.
+Require Import String.
+Require Import Arith.
+
+Require Import QuickChick.QuickChick.
+Import QcDefaultNotation. Open Scope qc_scope.
+
+Require Import Vminus.Atom.
+Require Import Vminus.CompilImp.
+Require Import Vminus.Vminus.
+Require Import Vminus.OpSemEval.
+
+Require Import Vminus.Imp.
+Require Import Vminus.ImpQuickChick.
+Require Import Vminus.VminusQuickChick.
+Require Import Vminus.CompilImpQuickChick.
+
+(** ** QuickChick and Vellvm **************************************************)
+(** One may expect a compiler for a language as simple as IMP to be relatively 
+    straightforward, and a proof of its correctness to be correspondingly
+    so. However, LLVM is a full-featured IR, and a faithful formalization 
+    is necessarily complex and large. When the compiler is under development, 
+    even stating the correctness of the compiler can be difficult, much 
+    less prove it.
+
+    But if we have interpreters for both the source and target, testing the 
+    compiler is a much simpler affair. Moreover, the simplicity of the source 
+    language, i.e. Imp. means that it is really easy to test! *)
+
+(** Following the lecture on compiler correctness, the first step is to define
+    what it means for an Imp state and an LLVM "state" to be equivalent. 
+    For correct compilation, it should be that all variables in the Imp state
+    can be mapped to their corresponding entities in the LLVM "state" following
+    the compiler, and that their values are equal. 
+
+    In this case, Imp variables are simplified to exactly the LLVM memory addr. 
+    Equivalence is thus checked by taking an ordering of the Imp variables and
+    checking the value at each corresponding address. *)
+
+(** Hence we have the following. *)
+
+
+(*
+(** Definition of a proper compiler, not correctness in the sense of 
+    semantics-preserving translation *)
+Definition comp_correct (comp : ectmon (val * list insn))
+                        (eval : mem -> nat) : Prop :=
+  forall cs cs' g st is k v,
+    
+  (* uid, val, instruction *) (cs', (v, is)) = comp cs ->
+  insns_at_pc g (st_pc st) (is ++ k) ->
+  exists st',
+    st_mem st' = st_mem st /\
+    insns_at_pc g (st_pc st') k /\
+    star (Opsem.step g) st st' /\
+    ids_preserved cs st st' /\
+    good_return cs' v /\
+    ctx_incr cs cs' /\
+    eval_val (st_loc st') v = Some (eval (st_mem st)).
+
+Lemma comp_aexp_correct : forall (a:aexp),
+  comp_correct (comp_aexp a) (aeval a).
+
+Lemma comp_bop_correct : forall b comp1 comp2 eval1 eval2
+    (IHa1: comp_correct comp1 eval1)
+    (IHa2: comp_correct comp2 eval2),
+    comp_correct (comp_bop b comp1 comp2)
+                 (fun m => bop_denote b (eval1 m) (eval2 m)).
+
+Lemma comp_store_correct : 
+  forall g a v le lr cs st,
+  insns_at_pc g (block_entry le) (steval (comp_store a v lr) cs) ->
+  st_pc st = (block_entry le) ->
+  exists st',
+    plus (step g) st st' /\
+    st_pc st' = (block_entry lr) /\
+    st_mem st' = (Memory.update (st_mem st) v (aeval a (st_mem st))).
+  
+Lemma comp_cond_correct :
+  forall g cs b le l1 l2 st,
+  insns_at_pc g (block_entry le) (steval (comp_cond b l1 l2) cs) ->
+  st_pc st = (block_entry le) ->
+  exists st',
+    plus (step g) st st' /\
+    st_pc st' = block_entry (if beval b (st_mem st) then l1 else l2) /\
+    st_mem st = st_mem st'.
+*)
+
+(*
+  (* plug in any cfg and initial execution state such that instructions at the 
+     current pc has instructions is ++ k. Then there exists an intermediate
+     state whose memory is the same as the initial, the instructions at this
+     new pc is just k, we can step from st to st', ids are preserved, 
+     ... 
+
+     So we need generators for:
+     - instructions, for extraneous k
+     - states, in particular program counters to place the instructions at
+     - 
+     And we need to:
+     - construct a dummy CFG g where instructions are placed in a given 
+       block, and which tell us where the cut-point target pc is.
+     - execute instructions from an initial state until this intermediate 
+       state is reached. 
+     - have a Checker for the conjunction of properties.  
+   *)
+*)
+
+Fixpoint memory_on_domain_checker
+         (dom: list addr) (st1 st2 : V.Opsem.state) : Checker :=
+  match dom with
+  | [] => checker true
+  | (a :: l) =>
+    if Nat.eqb (V.Opsem.st_mem st1 a) (V.Opsem.st_mem st2 a) then
+      memory_on_domain_checker l st1 st2
+    else
+      whenFail
+        ("memory_equal: memory at " ++ (Atom.string_of a)
+                                    ++ " not equal")%string
+        false
+  end.
+
+Fixpoint loc_on_domain_checker
+         (dom: list uid) (st1 st2 : V.Opsem.state) : Checker :=
+  match dom with
+  | [] => checker true
+  | (a :: l) =>
+    match V.Opsem.st_loc st1 a, V.Opsem.st_loc st2 a with
+    | Some n1, Some n2 =>
+      if Nat.eqb n1 n2 then loc_on_domain_checker l st1 st2
+      else whenFail "loc_equal: locs disagree" false
+    | None, None => loc_on_domain_checker l st1 st2
+    | _, _ => whenFail "loc_equal: locs disagree" false
+    end
+  end.
+
+Fixpoint insns_at_pc_checker `{Show pc}
+         (g: cfg) (p: pc) (k : list insn) : Checker :=
+  match k with
+  | [] => checker true
+  | (uid, cmd) :: instrs =>
+    match ListCFG.fetch g p with
+    | Some (uid', cmd') =>
+      if eq_dec_uid uid uid' then
+        if eq_dec_cmd cmd cmd' then insns_at_pc_checker g (incr_pc p) instrs
+        else whenFail ("insns_at_pc: cmd at pc "
+                         ++ (show p) ++ " not equal") false
+      else whenFail ("insns_at_pc: uid at pc "
+                       ++ (show p) ++ "not equal") false
+    | None => whenFail "insns_at_pc: cannot fetch" false
+    end
+  end.
+
+Definition eval_equal_checker
+           (eval: V.Opsem.mem -> nat) 
+           (st: V.Opsem.state) (v: val)
+  : Checker :=
+  let run_result := V.Opsem.eval_val (V.Opsem.st_loc st) v in
+  let expected_result := eval (V.Opsem.st_mem st) in
+  match run_result with
+  | Some n =>
+    whenFail "eval_equal: evaluation value not the same"
+             (Nat.eqb n expected_result)
+  | None => whenFail "eval_equal: run did not obtain any value" false
+  end.
+
+Definition ids_preserved_checker (cs : list addr) (st st': V.Opsem.state)
+  : Checker := loc_on_domain_checker cs st st'.
+
+Definition expression_step_checker
+           (eval: V.Opsem.mem -> nat)
+           (g: cfg)
+           (initial_state final_state: V.Opsem.state)
+           (k: list insn) (end_of_expr: pc)
+           (cs cs': list addr)
+           (v : val) : Checker :=
+  conjoin [ids_preserved_checker cs initial_state final_state;
+             insns_at_pc_checker g end_of_expr k;
+             eval_equal_checker eval final_state v].  
+(*
+    good_return cs' v /\
+    ctx_incr cs cs'
+ *)
+
+Fixpoint generate_dummy_insns (n : nat) : list insn :=
+  let fixed_addr := Atom.fresh [] in
+  let fixed_uid := Atom.fresh [] in
+  match n with
+  | 0 => []
+  | S n' =>
+    (fixed_uid, cmd_load fixed_addr) :: generate_dummy_insns n'
+  end.
+
+Definition wrap_code_in_cfg (p: pc) (instrs instrs_after: list insn)
+  : cfg * pc :=
+  let empty_cfg := [] in
+  let '(lbl, offset) := p in
+  let blocks :=
+      ListCFG.update empty_cfg lbl
+                     ((generate_dummy_insns offset)
+                        ++ instrs ++ instrs_after) in
+  ((lbl, blocks), (lbl, offset + List.length instrs)).
+
+Definition comp_correct_checker_inner
+           (comp: ectmon (val * list insn)) (eval: V.Opsem.mem -> nat)
+           (cs : list uid) (st: V.Opsem.state) (k: list insn)
+  : Checker :=
+  let '(cs', (v, instrs)) := comp cs in
+  let '(g, cutpoint) := wrap_code_in_cfg (V.Opsem.st_pc st) instrs k in
+  match eval_until_pc g st cutpoint 1000 with
+  | inl err => whenFail "evaluator failed" false
+  | inr st' => 
+    expression_step_checker eval g st st' k cutpoint cs cs' v
+  end.
+
+Definition comp_correct_checker
+           (comp: ectmon (val * list insn)) (eval: V.Opsem.mem -> nat)
+  : Checker :=
+  forAll arbitrary (fun (cs : list uid) =>
+  forAll arbitrary (fun (start_evaluation_state: state_with_meta) =>
+  forAll arbitrary (fun (extra_insn : list insn) =>
+    comp_correct_checker_inner
+      comp eval
+      cs (state_of start_evaluation_state) extra_insn))).
+
+(*
+Lemma comp_aexp_correct : forall (a:aexp),
+  comp_correct (comp_aexp a) (aeval a).
+*)
+Definition comp_aexp_correct_checker :=
+  forAll arbitrary (fun a: aexp =>
+    (comp_correct_checker (comp_aexp a) (aeval a))).
+
+(*! QuickChick comp_aexp_correct_checker. *)
+
+(*
+Lemma comp_bop_correct : forall b comp1 comp2 eval1 eval2
+    (IHa1: comp_correct comp1 eval1)
+    (IHa2: comp_correct comp2 eval2),
+    comp_correct (comp_bop b comp1 comp2)
+                 (fun m => bop_denote b (eval1 m) (eval2 m)).
+ *)
+
+Definition comp_bop_correct_checker: Checker :=
+  forAll arbitrary (fun (a1: aexp) =>
+  forAll arbitrary (fun (a2: aexp) =>
+  forAll arbitrary (fun (binop: bop) => 
+    comp_correct_checker 
+      (comp_bop binop (comp_aexp a1) (comp_aexp a2))
+      (fun m => V.Opsem.bop_denote binop (aeval a1 m) (aeval a2 m))))).
+
+(*! QuickChick comp_bop_correct_checker. *)
+
+(*
+  Lemma comp_store_correct : 
+  forall g a v le lr cs st,
+  insns_at_pc g (block_entry le) (steval (comp_store a v lr) cs) ->
+  st_pc st = (block_entry le) ->
+  exists st',
+    plus (step g) st st' /\
+    st_pc st' = (block_entry lr) /\
+    st_mem st' = (Memory.update (st_mem st) v (aeval a (st_mem st))).
+  
+Lemma comp_cond_correct :
+  forall g cs b le l1 l2 st,
+  insns_at_pc g (block_entry le) (steval (comp_cond b l1 l2) cs) ->
+  st_pc st = (block_entry le) ->
+  exists st',
+    plus (step g) st st' /\
+    st_pc st' = block_entry (if beval b (st_mem st) then l1 else l2) /\
+    st_mem st = st_mem st'.
+*)
+
+
+(*
+Inductive match_config : Imp.com -> (cfg * lbl * lbl) -> Prop :=
+  | MC_Skip : forall bs l,
+      match_config SKIP (bs, l, l)
+  | MC_Ass : forall g l l' uid a cs,
+      insns_at_pc g (block_entry l) (steval (comp_store a uid l') cs) ->
+      match_config (CAss uid a) (g, l, l')
+  | MC_Seq : forall g l1 l2 l3 c1 c2,
+      match_config c1 (g, l1, l2) ->
+      match_config c2 (g, l2, l3) ->
+      match_config (CSeq c1 c2) (g, l1, l3)
+  | MC_If : forall g le lr l1 l2 b c1 c2 cs,
+      match_config c1 (g, l1, lr) ->
+      match_config c2 (g, l2, lr) ->
+      insns_at_pc g (block_entry le) (steval (comp_cond b l1 l2) cs) ->
+      match_config (CIf b c1 c2) (g, le, lr)
+  | MC_While : forall g le lb lr b c cs,
+      match_config c (g, lb, le) ->
+      insns_at_pc g (block_entry le) (steval (comp_cond b lb lr) cs) ->
+      match_config (CWhile b c) (g, le, lr).
+
+Inductive match_states (g:cfg) (r:lbl)
+  : (com * Imp.state) -> Opsem.state -> Prop :=
+  match_states_intro : forall c mem st l,
+    match_config c (g, l, r) ->
+    st_pc st = block_entry l ->
+    st_mem st = mem ->
+    match_states g r (c, mem) st.
+
+Lemma transl_sim_step_final :
+  forall g r imp_st imp_st' vmn_st,
+  Imp.step imp_st imp_st' ->
+  match_states g r imp_st vmn_st ->
+  exists vmn_st',
+    (plus (Opsem.step g) vmn_st vmn_st' \/
+     star (Opsem.step g) vmn_st vmn_st' /\ imp_size imp_st' < imp_size imp_st) /\
+    match_states g r imp_st' vmn_st'.
+*)
